\documentclass[12pt]{article}
\usepackage{latexsym}
\usepackage{amssymb,amsmath,amsfonts}
\usepackage[pdftex]{graphicx}
\usepackage{color}

\topmargin = 0.1in \textwidth=5.7in \textheight=8.6in

\oddsidemargin = 0.2in \evensidemargin = 0.2in


\begin{document}

\begin{center}
    COMPUTER SCIENCE E-20, SPRING 2014 \\
    Check-in Problems \\
    Author: Tawheed Abdul-Raheem
\end{center}

\medskip


\begin{enumerate}
    \item Each of the following two claims and corresponding proofs is incorrect. For each one, explain why each proof is incorrect.
        \subitem (i) Claim: $1c = \$1$   \[ 1c = \$0.01= (\$ 0.1)^2 = (10c)^2 = 100c =\$1 \]
        \textbf{Solution: } 
        The propistion above holds true  until we got here:  
            \[ 1c = \$0.01= (\$ 0.1)^2 = (10c)^2 \] \[  (10c)^2 \neq (100c) \]
            \[  \therefore \text{our propistion is invalid this is because, } (10c)^2 = (100c)^2 \] 

        \subitem (ii) Claim: If $a=b$ then $a=0$\\ \[a=b\]\[a^2=ab\]\[a^2-b^2=ab-b^2\]\[(a-b)(a+b)=(a-b)b\]\[a+b=b\]\[a=0\]
        \textbf{Solution: } 
        The propistion above holds true  until we got here:  
            \[(a-b)(a+b)=(a-b)b\]
            This is because we are given the following in our propistion $a=b$ and it was said that if our propistion was true then $a = 0$, which also means that $a - b = 0$, however division by 0 leads to a mathematical error so our original claim does not hold

\end{enumerate}


\pagebreak


\end{document}
