\documentclass[12pt]{article}
\usepackage{latexsym}
\usepackage{amssymb,amsmath}
\usepackage[pdftex]{graphicx}
\usepackage{hyperref}
\usepackage{color}

\topmargin = 0.1in \textwidth=5.7in \textheight=8.6in
\oddsidemargin = 0.2in \evensidemargin = 0.2in

\begin{document}
\begin{center}
COMPUTER SCIENCE 20, SPRING 2014 \\
\smallskip

Module \#3 (Induction I)\\
Author: Tawheed Abdul-Raheem\\
\end{center}
\medskip



Use induction to prove that for all nonnegative integers $n$:
\[ \sum_{k=0}^{n}k^{2}=\frac{n(n+1)(2n+1)}{6} \]
\textbf{Solution: } We are going to use induction to prove
\[ \sum_{k=0}^{n}k^{2}=\frac{n(n+1)(2n+1)}{6} \]
for all nonnegative integers $n$ \\
\textbf{base case: } We prove when $n$ is $0$
\[ \sum_{k=0}^{n}k^{2}=\frac{n(n+1)(2n+1)}{6} \]
\[ \sum_{k=0}^{n}0^{2}=\frac{0(0+1)(2(0)+1)}{6} \]
\[0^2 = \frac{0}{6} \]
\textbf{Inductive step: } We prove that it is true for $n+1$, first we will solve
the left hand side of our equation
\[ \sum_{k=0}^{n}k^{2}=\frac{n(n+1)(2n+1)}{6} \]
\[ \sum_{k=0}^{n+1}k^{2}=\frac{(n+1)(n+2)(2(n+1)+1)}{6} \]
\[ \sum_{k=0}^{n}k^{2} + (n+1)^{2}=\frac{(n+1)(n+2)(2(n+1)+1)}{6} \]
\[ \frac{n(n+1)(2n+1)}{6}+(n+1)^{2}=\frac{(n+1)(n+2)(2n+2+1)}{6} \]
\[ \frac{n(n+1)(2n+1)+6(n+1)^{2}}{6}=\frac{(n+1)(n+2)(2n+3)}{6} \]
\[ \frac{(n+1)[(n)(2n+1)+6(n+1)]}{6}=\frac{(n+1)(n+2)(2n+3)}{6} \]
\[ \frac{(n+1)[(2n^{2}+7n+6)]}{6}=\frac{(n+1)(n+2)(2n+3)}{6} \]
\[ \frac{(n+1)(2n^{2}+7n+6)}{6}=\frac{(n+1)(2n^{2}+7n + 6)}{6} \]
\textbf{Then: } $P(n)$ is true for all nonnegative integers $n$


\end{document}
